\documentclass[13pt]{article}
\usepackage[margin=0.75in]{geometry}
\usepackage{amsmath,amssymb,amsfonts}
\usepackage{graphicx}
%opening
\title{}
\author{}

\begin{document}

\maketitle

Suppose $t_1$ and $t_2$ are two points in the domain of the curve with $t_2 > t_1$. We want expression for the distance between the points $(x(t_2), y(t_2))$ and $(x(t_1), y(t_1))$.


That is we want to evaluate

\[
	\Delta s = \sqrt{ \left( x(t_2) - x(t_1) \right)^2 + \left( y(t_2) - y(t_1) \right)^2 }
\]

From the mean value theorem we have that there exits a $t_x \in [t_1, t_2]$ such that

\begin{eqnarray*}
	\Delta x &=& x(t_2) - x(t_1) \\
	         &=& \frac{dx(t_x)}{dt}(t_2-t_1) \\
	         &=& \frac{dx(t_x)}{dt} \Delta t
\end{eqnarray*}

where 

\[
\frac{dx(t_x)}{dt} = \frac{dx}{dt}\bigg|_{t=t_x}
\]
and $\Delta t = t_2-t_1$.

Similarly for $y$ there exists a value $t_y \in [t_1, t_2]$ such that 

\begin{eqnarray*}
	\Delta y &=& y(t_2) - y(t_1) \\
	&=& \frac{dy(t_y)}{dt}(t_2-t_1) \\
	&=& \frac{dy(t_y)}{dt} \Delta t
\end{eqnarray*}

Thus we have

\[
	\Delta s = \sqrt{ \left(  \frac{dx(t_x)}{dt} \right)^2 + \left( \frac{dy(t_y)}{dt} \right)^2 } \Delta t
\]
But to get the Riemann sum we need the differential to be evaluated at the points $(x(t_1), y(t_1))$.
\begin{eqnarray*}
\Delta s &=& \sqrt{ \left(  \frac{dx(t_x)}{dt} \right)^2 + \left( \frac{dy(t_y)}{dt} \right)^2 } \Delta t \\
         &=& \sqrt{ \left(  \frac{dx(t_1)}{dt} \right)^2 + \left( \frac{dy(t_1)}{dt} \right)^2 } (t_2-t_1) + \epsilon(t_1, t_2)
\end{eqnarray*}

where 
\[
	\epsilon(t_1, t_2) = \sqrt{ \left(  \frac{dx(t_x)}{dt} \right)^2 + \left( \frac{dy(t_y)}{dt} \right)^2 } - \sqrt{ \left(  \frac{dx(t_1)}{dt} \right)^2 + \left( \frac{dy(t_1)}{dt} \right)^2 }
\]

Now we have 
\begin{eqnarray*}
	\left| \epsilon(t_1, t_2) \right| &=& \left|\sqrt{ \left(  \frac{dx(t_x)}{dt} \right)^2 + \left( \frac{dy(t_y)}{dt} \right)^2 } - \sqrt{ \left(  \frac{dx(t_1)}{dt} \right)^2 + \left( \frac{dy(t_1)}{dt} \right)^2 } \right| \\
		                  &\le& \sqrt{\left(\frac{dx(t_x)}{dt} - \frac{dx(t_1)}{dt} \right) ^ 2 + \left(\frac{dy(t_y)}{dt} - \frac{dy(t_1)}{dt} \right) ^ 2}  \\
		                  &\le& \left| \frac{dx(t_x)}{dt} - \frac{dx(t_1)}{dt} \right| + \left| \frac{dy(t_y)}{dt} - \frac{dy(t_1)}{dt} \right|
\end{eqnarray*}
where the first inequality comes from the reverse triangle inequality  $\left| \left|a\right| - \left|b\right| \right| \le \left| a-b \right|$ and the second comes from the regular triangle inequality $\left| a+b \right| \le \left|a\right| + \left|b\right|$. 

Finally the first derivatives of $x$ and $y$ are continuous we can make $\epsilon(t_1, t_2)$ arbitrary small as we let $\Delta t$ become small.




\end{document}
